\input{preamble/preamble_ask.tex}
\input{preamble/definitions.tex}


\thispagestyle{empty}

\begin{document}

\begin{center}
    \minibox[frame]{\large\bfseries ΣΔΕ Τύπου Euler}
\end{center}

\vspace{\baselineskip}

\begin{enumerate}
    \item Να λυθούν οι παρακάτω σδε τύπου Euler.
        \begin{enumerate}[i)]
            \setlength\itemsep{15pt}
        \item $ x^{2}y''(x)-3xy'(x)+3y(x)=0 $ 
            \hfill Απ: $ y(x)=c_{1}x + c_{2}x^{3} $
        \item $ x^{2}y''(x)-2xy'(x)-4y(x)=0 $,\; $ x \neq 0 $ 
            \hfill Απ: $ y(x)=c_{1}x^{4}+ c_{2} x^{-1} $ 
        \item $ x^{2}y''(x)-xy'(x)+y(x)=1 $,\; $ x>0 $ 
            \hfill Απ: $ y(x)=(c_{1}+c_{2} \ln{x})x + 1 $  
        \item $ x^{2}y''(x)-3xy'(x)-5y(x)=x^{3} $ 
            \hfill Απ: $ y(x)=c_{1}x^{5}+ c_{2} x^{-1}- \frac{x^{3}}{8} $ 
        \item $ x^{2}y''(x)+xy'(x)-y(x)=x^{4} $ 
            \hfill Απ: $ y(x)=c_{1}x+c_{2}x^{-1}+ \frac{x^{4}}{15} $ 
        \item \label{eul} $ (x+3)^{2}y''(x)+3(x+3)y'(x)+y(x)=0 $,\; $ x>-3 $ 
            \hfill Απ: $\scriptstyle{ c_{1} (x+3)^{-1} + c_{2}\ln(x+3)(x+3)^{-1}} $
        \end{enumerate}

    \item Να λυθούν οι παρακάτω σδε με τη βοήθεια της μεθόδου υποβιβασμού τάξης.
        \begin{enumerate}[i)]
            \setlength\itemsep{15pt}
        \item $ y'' + \tan{x} y' = 0 $ \hfill Απ: $ y= c_{1} \sin{x} + c_{2} $ 
        \item $ 2x^{2}y''+ (y')^{3} = 2xy $ 
            \hfill Απ: $ y= \frac{2}{3} \sqrt{x+c_{1}}^{3} - 
            2c \sqrt{x+c_{1}} + c_{2} $ 
        \item $ (1+x^{2})y'' + 2xy' = 2x^{-3} $ \hfill Απ: $ y= \frac{1}{x} 
            \arctan x + c_{1} \arctan x + c_{2} $ 
        \end{enumerate}
\end{enumerate}

\end{document}
