\documentclass[a4paper,table]{report}
\input{preamble_ask.tex}
\input{definitions_ask.tex}

% \everymath{\displaystyle}
\pagestyle{vangelis}

\begin{document}


\begin{center}
  \minibox{\large\bfseries  \textcolor{Col1}{Εξισώσεις}}
\end{center}

\subsection*{1ου βαθμού}

\begin{enumerate}
  %papadakis p180
  \item  Να λυθούν οι παρακάτω εξισώσεις.
    \begin{enumerate}[i)]
      \item $ 6x-2=9x-5 $ \hfill Απ: $ x=1 $
      \item $ 3(x+4)-(x-2) = 2+x $ \hfill Απ: $ x=-12 $ 
      \item $ 3(2x+1) - 14 = 2(3x+5) $ \hfill Απ: αδύνατη 
      \item $ 10x-2(4+5x) =-8 $ \hfill Απ: ταυτότητα 
    \end{enumerate}

  \item  Να λυθούν οι παρακάτω εξισώσεις.
    \begin{enumerate}[i)]
      \item $ \frac{x-2}{3} = \frac{9-x}{4} $ \hfill Απ: $ x=5 $ 
      \item $ 3 - \frac{x+2}{4} = x+10 $ \hfill Απ: $ x=-6 $ 
      \item $ \frac{x-2}{4} - \frac{x-3}{2} = \frac{2-x}{3} $ \hfill Απ: $ x=-4 $ 
      \item $ \frac{1}{3} - \frac{2(x-1)}{9} = \frac{x+5}{18} $ \hfill Απ: $ x=1 $ 
      \item $ \frac{x+4}{2} - \frac{5-x}{3} = x - \frac{x-2}{6} $ \hfill Απ: ταυτότητα
      \item $ \frac{3x-2}{4} - \frac{x+1}{2} = 3 - \frac{3-x}{4} $ \hfill Απ: αδύνατη 
    \end{enumerate}
\end{enumerate}

\subsection*{2ου βαθμού}

\begin{enumerate}
  \item  Να λυθούν οι παρακάτω εξισώσεις.
    \begin{enumerate}[i)]
      \item $ x^{2} + 5x + 4 = 0 $ \hfill Απ:  $ -4, -1 $
      \item $ x^{2} - 10x + 25 = 0 $ \hfill Απ: $ 5 $
      \item $ x^{2} - 4x + 5 = 0 $ \hfill Απ:  αδύνατη
      \item $ -x^{2} - 8x + 9 = 0 $ \hfill Απ: $ -9, 1 $
      \item $ 4x^{2} + 20x + 25 = 0 $ \hfill Απ: $ - \frac{5}{2} $ 
    \end{enumerate}

  \item Να λυθούν οι παρακάτω εξισώσεις.
    \begin{enumerate}[i)]
      \item $ (x^{2} - 4)(x^{2} - 5x + 6) = 0 $ \hfill Απ: $ -2, 3, 2 $ 
      \item $ (x^{2} + 5x)(3x^{2} - 2x - 8) = 0 $ \hfill Απ: $ 0, -5, 2, -\frac{4}{3} $
      \item $ (x^{2} - 7x + 6)(4x^{2}- 8x + 3) = 0 $ \hfill Απ: $ 6, 1, \frac{1}{2},
        \frac{3}{2} $
      \item $ (9x^{2} - 6x + 1)(x^{2} - x - 2) = 0 $ \hfill Απ: $ \frac{1}{3}, 2, -1  $ 
    \end{enumerate}

  \item Να λυθούν οι παρακάτω εξισώσεις.
    \begin{enumerate}[i)]
      \item $ 3x^{2} - 2x + 1 = 2 $ \hfill Απ: $ 1, - \frac{1}{3} $  
      \item $ 3x^{2} + 2x - 4 = 3x - 7 $ \hfill Απ:  αδύνατη
      \item $ 4x^{2} - 6x + 5 = 4 - 5x^{2} $ \hfill Απ: $ \frac{1}{3} $
      \item $ 5x^{2} - 3x = 2x + x^{2} - 1 $ \hfill Απ: $ \frac{1}{4}, 1 $ 
    \end{enumerate}

  \item Να λυθούν οι παρακάτω εξισώσεις.
    \begin{enumerate}[i)]
      \item $ (x-1)(x-2) = x(x-4)+(x+2)^{2} $ \hfill Απ: $ -1, -2 $
      \item $ (2x-1)^{2} - (x-3)^{2} = (x+1)(2x-1) - 1 $ \hfill Απ: $ 2, -3 $
      \item $ (2-x)^{2} - (x-1)(x+1) = (x+3)^{2} - 6x $ \hfill Απ: $ -2 $
      \item $ 2(x-2)(x+3) + (-x-1)^{2} = (x-1)^{2} - (x-2)^{2} $ \hfill Απ: $ -2,
        \frac{4}{3} $ 
    \end{enumerate}

  \item Να λυθούν οι παρακάτω εξισώσεις.
    \begin{enumerate}[i)]
      \item $ \frac{x^{2}}{6} - \frac{2x}{3} = \frac{3x-10}{4} $ \hfill Απ: $
        \frac{5}{2}, 6 $
      \item $ \frac{x-2}{2} = \frac{(x-1)(x+1)}{3} - \frac{2x+1}{6} $ \hfill Απ: $
        \frac{3}{2}, 1 $ 
      \item $ \left(\frac{x-1}{2}\right)^{2} - \frac{2x}{5} = 
        \frac{2x+3}{2} - \frac{(5x-1)(2x+5)}{20} $ \hfill Απ: $ 2, -1 $ 
    \end{enumerate}
\end{enumerate}

\end{document}
