\input{preamble_ask.tex}
\input{definitions_ask.tex}

\geometry{top=1.5cm}
\everymath{\displaystyle}
\pagestyle{vangelis}

\begin{document}

\begin{center}
  \minibox{\bfseries\large \textcolor{Col1}{Ασκήσεις στις Παραγώγους}}
\end{center}

\vspace{\baselineskip}

\section{Όρια}

\begin{enumerate}
  \item $ \lim_{x \to 0} \frac{\sqrt{x+1} -1 - \frac{x}{2}}{x^{2}} $ 
    \hfill Απ: $ -\frac{1}{8} $ 
  \item $ \lim_{x \to \infty} \frac{a \ln{(bx+c)}}{x}, \quad a,b,c > 0 $ 
    \hfill Απ: $ 0 $ 
  % \item $ \lim_{x \to \infty} \frac{x^{n}}{\mathrm{e}^{x}} $ \hfill Απ: 0 
  \item $ \lim_{x \to 0} \left(\frac{1}{x} - \frac{1}{\mathrm{e}^{x} -1}\right) $ 
    \hfill Απ: $ \frac{1}{2} $
  \item $ \lim_{x \to 1^{+}} (x-1)^{\ln{x}} $ \hfill Απ: $ 1 $ 
\end{enumerate}

\section{Παράγωγος}

\begin{enumerate}
  \item $ f(x) = \frac{\ln{x}}{\mathrm{e}^{x^{2}}} $ \hfill Απ: $ \frac{1}{x}
    (\mathrm{e}^{-x^{2}} - 2x^{2} \mathrm{e}^{-x^{2}} \ln{x}) $ 
  \item $ g(x) = x^{x} $ \hfill Απ: $ x^{x}(\ln{x} + 1) $  
  \item $ h(x) = xa^{2x+4} $ \hfill Απ: $ a^{2x+4}(2x \ln{a} + 1) $ 
  \item $ f(x) = \sqrt{xa^{2x+4}}$ 
    \hfill Απ: $ \frac{a^{2x+4}(2x \ln{a} + 1)}{2 \sqrt{xa^{2x+4}}} $ 
  \item $ u(x) = \sqrt{(x-1)^{5}(6x-5)} $ 
    \hfill Απ: $ \frac{(36x-31)(x-1)^{4}}{2 \sqrt{(6x-5)(x-1)^{5}}} $ 
  \item $ v(x) = \sin{(2x^{2}+ \cos(2x)+1)} $ 
    \hfill Απ: $ \cos{(2x^{2} + \cos{2x} +1)} (4x - 2 \sin{2x}) $ 
\end{enumerate}

\section{Αλυσιδα}

\begin{enumerate}
  \item $ y = \sqrt{\ln{(\mathrm{e}^{x} + 2x + 5)}} $ 
    \hfill Απ: $ \frac{\mathrm{e}^{x} + 2}{2 \sqrt{\ln{(2x+ \mathrm{e}^{x} + 5) 
    (\mathrm{e}^{x} + 2x+5)}}} $
\end{enumerate}


\end{document}
