\input{preamble_ask.tex}
\input{definitions_ask.tex}

\pagestyle{askhseis}

\begin{document}



\begin{center}
  \minibox{\large \bfseries \color{Col1} Ασκήσεις ΣΔΕ (1ης τάξης)}
\end{center}

\vspace{\baselineskip}

\begin{enumerate}
  \item {\bfseries Να λυθούν οι παρακάτω σδε: (Χωριζομένων Μεταβλητών)}
    \begin{enumerate}[i)]
      \item $ y' = - \frac{y}{x} $, \quad $ y(1)=1 $ \hfill Απ: $ y = \frac{1}{x} $ 
      \item $ y'- \frac{y}{x} = y $ \hfill Απ: $ y=cx \mathrm{e}^{x} $ 
      \item $ 2xy'+y^{2} = 1 $ \hfill Απ: $ y= \frac{cx-1}{cx+1} $ 
      \item $ y'=1+y^{2} $ \hfill Απ: $ y= \tan{x+c} $ 
    \end{enumerate}

  \item {\bfseries Να λυθούν οι παρακάτω σδε: (Γραμμικές)}
    \begin{enumerate}[i)]
      \item $y'=\frac{y}{x-1}+x^2-1$\hfill Απ: $y=(x-1)\Bigl[c+\frac{x^2}{2}+x\Bigr]$
      \item $y'=\frac{y}{x}+x\cos x$\hfill Απ: $y=x[c+\sin x]$
        % \item $y'=2xy+1$\hfill Απ: $y=e^{x^2}\Bigl[c+\frac{\sqrt{\pi}}{2}\erf(x)\Bigr]$
      \item $xy'=-2y+ \sin{x}$ \hfill Απ: $ y= - \frac{\cos{x}}{x} +
        \frac{\sin^{2}{x}}{x^{2}} + \frac{c}{x^{2}} $ 
        % \item $y'=\frac{1}{x+e^{2y}}$\hfill Απ: $x=ce^y+e^{2y}$
        % \item $ (y^{2}-x)y'=1 $ \hfill Απ: $ x = ce^{-y}+y^{2}-2y+2 $ 
      \item $ y'=-2xy+2x $, \quad $ y(0)=2 $ \hfill Απ: $ y=1+e^{-x^{2}} $  
    \end{enumerate}

  \item {\bfseries Να λυθούν οι παρακάτω σδε: \textlatin{(Bernoulli)}}
    \begin{enumerate}[i)]
      \item $y'=-xy+xy^2$\hfill Απ: $y=\frac{1}{-e^{\frac{x^2}{2}}+1}$
      \item $2yy'-xy^2=x^3$\hfill Απ: $y^2=ce^{\frac{x^2}{2}}-(x^2+2)$
      \item $y'+y=y^{\frac{2}{3}}$ \hfill Απ: $y^{\frac{1}{3}}=1+ce^{-\frac{x}{3}}$
        % \item $ y'=y- \frac{1}{4} y^{\frac{3}{2}} $ 
        %   \hfill Απ: $ y= \frac{1}{(ce^{- \frac{x}{2}}+ \frac{1}{4} )^{2}}  $ 
      \item $xy'+y=y^{2}\ln x \quad y(e)=1$ \hfill Απ: $y^{-1}=-xe^{-1}+1+\ln x$
      \item $ y'+2xy=2x^{3}y^{3} $, \quad $ y(0)=1 $ 
        \hfill Απ: $ y=\frac{1}{\sqrt{x^{2}+ \frac{1}{2}+\frac{1}{2} e^{2x^{2}}}} $ 
    \end{enumerate}


    % \item {\bfseries Να λυθουν οι παρακατω σδε: (Riccati)}
    %   \begin{enumerate}[i)]
    %     \item $y'=y^2-2xy+x^2+1,\quad y_0=x$\hfill Απ: $y=x+\frac{1}{-x+c}$
    %     \item $ y' = \frac{1}{x^{3}}y^{2} - \frac{1}{x}y + 2x $, $ x>0 $,
    %       \quad $ y_{0}=x^{2} $ \hfill Απ: $ y=x^{2}\left(\frac{2+cx}{1+cx}\right) $ 
    %     \item $ 4y'+y^{2}+ \frac{4}{x^{2}} = 0 $,\quad $ y_{0} = \frac{2}{x} $ 
    %       \hfill Απ: $ y =\frac{2}{x}+\frac{1}{x\left(x+\frac{1}{4} \ln{x}\right)} $  
    %     \item $y'=\frac{2}{x}y^2+\frac{1}{x}y-x$
    %       \hfill Απ: $y=x\left(\frac{1}{2}\cdot\frac{1+ce^{2x}}{1-ce^{2x}}\right)$
    %   \end{enumerate}

  \item {\bfseries Να λυθούν οι παρακάτω σδε: (Ομογενείς)}
    \begin{enumerate}[i)]
      \item $y'=\frac{y}{x}+\sin(\frac{y}{x}), \quad x\neq 0,\; y\neq k\pi x$ 
        \hfill Απ: $y=2x\arctan(c_{1}x)$
      \item $y'=-\frac{2x+y}{x+2y}, \quad x\neq 0,\; y\neq 0$  
        \hfill Απ: $y^{2}+xy+x^{2}=c$
      \item $x^{2}y'+y^{2}=xy, \quad x>0,\; y\neq 0$ \hfill Απ:$\frac{x}{y}=\ln x+c$
      \item $\left(xe^{\frac{y}{x}}+y\right)dx=xdy, \quad x>0$ 
        \hfill Απ: $e^{-\frac{y}{x}}+\ln x =c$
      \item $ xy'=y(\ln{y} - \ln{x} +1) $, $ x,y>0 $ \hfill Απ: $ y=xe^{cx} $ 
        % \item $ y' = \frac{y}{x+y \sin^{2}{(\frac{y}{x})}} $ 
        %   \hfill Απ: $ y=ce^{- \cot{\frac{x}{y} }} $  
        % \item $ xy' = \sqrt{ x^{2}-y^{2} } +y $, \quad $ y(1)=0 $ 
        %   \hfill Απ: $ y = x \sin{(\ln{x})}$  
    \end{enumerate}

  \item {\bfseries Να λυθούν οι παρακάτω σδε: (ακριβείς)}
    \begin{enumerate}[i)]
      \item $ (3x^{2}+2y^{2})dx+(4xy+6y^{2})dy=0  $ 
        \hfill Απ: $ x^{3}+2xy^{2}+2y^{3}=c $ 
      \item $(3x^2+6xy^2)dx+(6x^2y+4y^3)dy=0$\hfill Απ: $x^3+3x^2y^2+y^4=c$
      \item $ (\cos{x} + \ln{y})dx + \left(\frac{x}{y} + e^{y}\right)dy=0 $ 
        \hfill Απ: $ \sin{x} + x \ln{y} + e^{y}=c $ 
      \item $ y'=- \frac{x^{3}+3xy^{2}}{3x^{2}y+y^{3}} $ 
        \hfill Απ: $ \frac{x^{4}}{4}+\frac{3}{2} x^{2}y^{2}+\frac{y^{4}}{4} = c $ 
      \item $\left(4x^3y^3+\frac{1}{x}\right)dx+\left(3x^4y^2-
        \frac{1}{y}\right)dy=0, \quad x(e)=1$
        \hfill Απ: $x^4y^3+\ln \Bigl|\frac{x}{y}\Bigr|=e^3-1$
      \item $ -2xdy + (3x^{2}-2y)dx=0 $, \quad $ y(1)=0 $ 
        \hfill Απ: $ y= \frac{x^{3}-1}{2x} $ 
        % \item $ x y' = 2x \mathrm{e}^{x} -y+6x^{2} $ 
        % \hfill Απ: $ 2 \mathrm{e}^{x} - 2x \mathrm{e}^{x} - 2x^{3} + xy=c $ 
    \end{enumerate}

\end{enumerate}

\end{document}
