\input{preamble.tex}
\input{definitions_ask.tex}

\pagestyle{askhseis}
\everymath{\displaystyle}

\begin{document}



\begin{center}
  \minibox[c]{\large \bfseries \color{Col1} Ασκήσεις ΣΔΕ \\ \large \bfseries
  \textcolor{Col1}{(Μέθοδος Σειρών)}}
\end{center}

\vspace{\baselineskip}

\begin{enumerate}
  \item Να λυθούν, με τη μέθοδο των σειρών, κοντά στο σημείο $ x_{0}=0 $, οι παρακάτω 
    εξισώσεις.
    \begin{enumerate}[i)]
      \item $ y'=y $
        \hfill Απ: $ y= a_{0}e^{x} $ 

      \item $ (1+x)y'-3y=0 $
        \hfill Απ: $ y= a_{0}(1+x)^{3} $ 

      \item $ x y'-3y=3 $ %Frobenious
        \hfill Απ: $ y= - 1 + a_{3} x^{3} $ 

      \item $ y''+y=0 $ %omalo
        \hfill Απ: $ y= a_{0} \cos{x} + a_{1} \sin{x} $

      \item $ y'' + x^{2}y = 0 $ %omalo
        \hfill Απ: $ y= a_{0}\Bigl(1- \frac{x^{4}}{12} + \frac{x^{8}}{672} - 
          \cdots\Bigr) + a_{1} \Bigl(x - \frac{x^{5}}{20} + \frac{x^{9}}{1440} - 
        \cdots\Bigr) $ 

      \item $ y'' -xy'+2y=0 $ %omalo
        \hfill Απ: $ y = a_{0}\Bigl(1-x^{2}\Bigr) + a_{1}
        \Bigl(x - \frac{x^{3}}{6} - \frac{x^{5}}{120} - \frac{x^{7}}{1680} - 
        \cdots \Bigr) $ 

      \item  $ x^{2}y'' - 2.5 x y' -2y=0 $ \quad (Euler-Cauchy) %Frobenious (1h per)
        \hfill Απ: $ y = c_{1}x^{-0.5}+ c_{2}x^{4} $ 

      \item $ x(x-1)y''+(3x-1)y'+y=0 $ %Frobenious (2h per) 
        \hfill Απ: $ y= c_{1} \frac{1}{1-x} + c_{2} \frac{\ln{x}}{1-x}, 
        \quad \abs{x} <1$ 

      \item $ (x^{2}-x)y'' -xy'+y=0 $ %Frobenious (3h per)
        \hfill Απ:  $ y= c_{1}x + c_{2}(x \ln{x} + 1) $

      \item $ x^{2}y''-xy'+y=0 $ \quad (Euler-Cauchy) %Frobenious (2h per)
        \hfill Απ: $ y= c_{1}x + c_{2}x \ln{x} $ 

      \item $y''+x^2y'-4xy=0$
        \hfill Απ:
        $y= a_{0}\Bigl(x+\frac{1}{4}x^4\Bigr) + a_{1}\Bigl(1+\frac{2}{3}x^3+\frac{1}
        {4\cdot 5}x^6- \frac{1}{16\cdot 20}x^9+\cdots\Bigr) $

      \item $2xy''-y'+x^{2}y=0 $
        \hfill Απ:  $ y= c_{1}\Bigl(1- \frac{1}{27} x^{3+ \frac{3}{2}} + 
        \frac{1}{2430} x^{6+ \frac{3}{2} } + \cdots\Bigr) + 
        c_{2}\Bigl(1 - \frac{1}{9} x^{3} + \frac{1}{486} x^{6} + \cdots \Bigr) $

      \item $xy''+2y'-xy=0$
        \hfill Απ: 
        $y= c_{1}\frac{\cosh x}{x} + c_{2}\frac{\sinh x}{x}$
    \end{enumerate}

  \item Να λυθεί, με τη μέθοδο των σειρών, κοντά στο σημείο $ x_{0}=1 $, η παρακάτω
    εξισώση. \textcolor{Col1}{Υπόδειξη}: θέτουμε $ t=x- x_{0} $
    \[ 
      (2-x)y'' + y=0 
    \]

    \hfill Απ: $ y= c_{1}\Bigl((x-1)- \frac{1}{6} (x-1)^{3}- \frac{1}{12} (x-1)^{4} 
      + \cdots\Bigr) + c_{2}\Bigl(1- \frac{1}{2} (x-1)^{2} - \frac{1}{6} (x-1)^{3} 
    - \frac{1}{24} (x-1)^{4} + \cdots \Bigr) $  
\end{enumerate}




\end{document}
