\input{preamble_ask.tex}
\input{definitions_ask.tex}

\pagestyle{askhseis}
\everymath{\displaystyle}

\begin{document}



\begin{center}
  \minibox{\large \bfseries \color{Col1} Ασκήσεις ΣΔΕ (2ης ταξης)} 
  % από σημειώσεις Πανδή
\end{center}

\vspace{\baselineskip}

\begin{enumerate}
  \item Να βρεθεί η γενική λύση των παρακάτω σδε.
    \begin{enumerate}[i)]
      \item $ x^{2}y'' - xy' + y = 0 $ \hfill Απ: $ y_{1}=x, \; y_{2} = x \ln{x} $ 
    \end{enumerate}

  \item Να βρεθεί η γενική λύση των παρακάτω σδε.
    \begin{enumerate}[i)]
      \item $ y'' - y=0 $, \quad $ y(0)=4, \; y'(0)=-5 $ 
        \hfill Απ:  $ y= \mathrm{e}^{x}+3 \mathrm{e}^{-2x} $ 
      \item $ y''-4y'+4y=0 $, \quad $ y(0)=3, \; y'(0)=1 $ 
        \hfill Απ:  $ y=3 \mathrm{e}^{2x} - 5x \mathrm{e}^{2x} $
    \end{enumerate}

  \item Να βρεθεί η γενική λύση των παρακάτω σδε.
    \begin{enumerate}[i)]
      \item $ y''+4y=8x^{2} $, \quad $ y(0)=-1, \; y'(0)=2 $ 
        \hfill Απ: $ y= \sin{2x} + 2x^{2}-1 $ 
      \item $ y''-3y'+2y= \mathrm{e}^{x} $
        \hfill Απ: $ y= c_{1} \mathrm{e}^{2x} + c_{2} \mathrm{e}^{x} - x
        \mathrm{e}^{x}  $ 
      \item $ (1+x^{2})y''-2xy'+2y=2x $ 

        \hfill Απ: $ y= c_{1}x + c_{2}(x^{2}-1) - x \ln{(x^{2}+1)} - \frac{2x}{x^{2}+1}
        + (x^{2}-1) \arctan(x) - \frac{x(x^{2}-1)}{x^{2}+1} $
    \end{enumerate}
\end{enumerate}





\end{document}
