\input{preamble_ask.tex}
\input{definitions_ask.tex}


\pagestyle{askhseis}

\begin{document}


\begin{center}
  \minibox{\large \bfseries \textcolor{Col1}{Διαφορικές Εξισώσεις}}
\end{center}

\vspace{\baselineskip}

\section*{Χωριζομένων Μεταβλητών}


\begin{enumerate}
  \item Να λυθούν οι παρακάτω διαφορικές εξισώσεις.
    \begin{enumerate}[i)]
      \item $ y' =\frac{x^2}{y^2}$, όπου $ y=y(x) $ 
        \hfill Απ: $y^3=x^3+c$
      \item $y'=y^2\cos x$, όπου $ y=y(x) $ \hfill Απ: $y=-\frac{1}{\sin x +c }$
      \item $ y' =\frac{6x^2}{2y+\cos y}$, αν $ y=y(x) $ 
        \hfill Απ: $y^2+\sin y = 2x^3 +c$
      \item $ y(xy'-y)=2 $, όπου $ y=y(x) $ 
        \hfill Απ: $ y^2=cx^2-2 $   
      \item $ xdy- \sqrt{1+y^2} dx=0 $, όπου ν $ y=y(x) $ 
        \hfill Απ: $ y+ \sqrt{1+y^2} = cx $  
      \item $ \mathrm{e}^{x} dx - ydy = 0 $, όπου $ y=y(x) $ 
        και $ y(0)=1 $. \hfill Απ: $ y^{2} = \sqrt{2 \mathrm{e}^{x} + c}$
      \item $ xdx-y^{2}dy=0  $, όπου $ y=y(x) $ 
        \hfill Απ: $ y= \sqrt[3]{\frac{3x^{2}+c}{2}}  $
      \item $xydx + (x+1)dy=0$, όπου $ y=y(x) $ \hfill Απ: $x-\ln|x+1|+\ln|y|=c$
      \item $(x+x^2)y'=y+2xy$, όπου $ y=y(x) $ \hfill Απ: $y=cx(1+x)$
      \item $4xydx+(x^2+1)dy=0$, όπου $ y=y(x) $ \hfill Απ: $y=\frac{c}{(1+x^2)}$
    \end{enumerate}
\end{enumerate}


\section*{Γραμμικές}

\begin{enumerate}
  \item Να λυθούν οι παρακάτω διαφορικές εξισώσεις.
    \begin{enumerate}[i)]
      \item $ xy'+y=3x^{2} $ \hfill Απ: $ y= \frac{c}{x} + x^{2} $  
      \item $ y'-2y= cosx $ \hfill Απ: $ y=c \mathrm{e}^{2x} + \frac{1}{5} (\sin{x}
        - 2 \cos{x}) $  
      \item $ 2xy'-3y=x^{2} $, όπου $ x>0 $ \hfill Απ: $ y=cx^{3/2} +x^{2} $ 
      \item $ y'-y=x \mathrm{e}^{x} $ \hfill Απ: $ y=c \mathrm{e}^{x} +
        \frac{\mathrm{e}^{x} x^{2}}{2} $ 
      \item $ y'- \frac{y}{x} -2x \sin{x} = 0 $, με $ y(\frac{\pi}{2}) = 0 $
        \hfill Απ: $ y=-2x \cos{x} $  
        \end{enumerate}
\end{enumerate}


\section*{Bernoulli}

\begin{enumerate}
  \item Να λυθούν οι παρακάτω διαφορικές εξισώσεις.
    \begin{enumerate}[i)]
      \item $ y'+xy=3xy^3$ \hfill Απ: $y^2= \frac{1}{c \mathrm{e}^{x^{2}} +3} $  
      \item $ y'+2xy=xy^2$ \hfill Απ: $y= \frac{2}{1+c \mathrm{e}^{x^2}}$  
      \item $ y'+ \frac{2}{x} y = xy^2$ \hfill Απ: $y= \frac{1}{x^{2}(c- \ln{x})} $ 
      \item $y'- \frac{4}{x} y = y^3$ \hfill Απ: $y^2= \frac{9x^8}{9c-2x^9} $ 
      \item $y'- \frac{6}{x} y = y^{1/3} $ \hfill Απ: $y^{2/3}=x^4(c- \frac{2}{9x^3})$
        \end{enumerate}
\end{enumerate}


\end{document}
